cleanq/rb: finished list -> rb weak frame condition proofs
Signed-off-by: Roni Häcki <roni.haecki@inf.ethz.ch>

CleanQ/CleanQ_RBModel.thy
@@ -217,25 +217,22 @@ text \<open>
   Assuming a two concurrently acting agents, we can not assume that all of the RB state
   stays the same. In order to model this, we have to weaken the frame condition which
   we up to now implicitly used. \<close>
-(*
+
 definition frame_rb_weak_x :: "'a CleanQ_RB_State \<Rightarrow> 'a CleanQ_RB_State \<Rightarrow> bool"
-  where "frame_rb_weak_x st' st \<longleftrightarrow> rSX st = rSX st' \<and> frame_rb_weak_left (rTXY st') (rTXY st) 
-                                    \<and> frame_rb_weak_right (rTYX st') (rTYX st) \<and> 
-                                    (rSY st' = (set (rb_delta_head_st (rTYX st') (rTYX st)) \<union> 
-                                     rSY st - set (rb_delta_tail_st (rTXY st') (rTXY st))))" 
-*)
-definition frame_rb_weak_x :: "'a CleanQ_RB_State \<Rightarrow> 'a CleanQ_RB_State \<Rightarrow> bool"
-  where "frame_rb_weak_x st' st \<longleftrightarrow> rSX st = rSX st' \<and> frame_rb_weak_left (rTXY st') (rTXY st) 
-                                    \<and> frame_rb_weak_right (rTYX st') (rTYX st) \<and> 
-                                    (rSY st' \<union> set (rb_delta_tail_st (rTXY st') (rTXY st)) = (set (rb_delta_head_st (rTYX st') (rTYX st)) \<union> 
-                                     rSY st) \<and> distinct (rb_delta_head_st (rTYX st') (rTYX st)))" 
+  where "frame_rb_weak_x st' st \<longleftrightarrow> rSX st = rSX st' \<and> frame_rb_weak_left (rTXY st') (rTXY st) \<and> 
+                                    frame_rb_weak_right (rTYX st') (rTYX st) \<and> 
+                                    rSY st' \<union> set (rb_delta_tail_st (rTXY st') (rTXY st)) = (set (rb_delta_head_st (rTYX st') (rTYX st)) \<union> 
+                                    rSY st) \<and> distinct (rb_delta_head_st (rTYX st') (rTYX st)) \<and> 
+                                    rSY st \<inter> set (rb_delta_head_st (rTYX st') (rTYX st)) = {}" 
 
 
 definition frame_rb_weak_y :: "'a CleanQ_RB_State \<Rightarrow> 'a CleanQ_RB_State \<Rightarrow> bool"
   where "frame_rb_weak_y st' st \<longleftrightarrow> rSY st = rSY st' \<and> frame_rb_weak_left (rTYX st') (rTYX st) \<and>
                                     frame_rb_weak_right (rTXY st') (rTXY st) \<and>
-                                    (rSX st' = (set (rb_delta_tail_st (rTYX st') (rTYX st)) \<union> 
-                                     rSX st - set (rb_delta_head_st (rTXY st') (rTXY st))))"
+                                    rSX st' \<union> set (rb_delta_tail_st (rTYX st') (rTYX st)) = (set (rb_delta_head_st (rTXY st') (rTXY st)) \<union> 
+                                    rSX st) \<and> distinct (rb_delta_head_st (rTXY st') (rTXY st)) \<and> 
+                                    rSX st \<inter> set (rb_delta_head_st (rTXY st') (rTXY st)) = {}" 
+
 
 lemma frame_rb_s_w_x:
  "frame_rb_strong st' st \<Longrightarrow> frame_rb_weak_x st' st"
@@ -251,7 +248,6 @@ lemma frame_rb_s_w_y:
   by (simp add: rb_delta_head_def rb_delta_tail_def rb_incr_head_n_delta_def 
       rb_incr_head_n_delta_map_def rb_incr_tail_n_delta_def rb_incr_tail_n_delta_map_def)
   
-
 
 (* ------------------------------------------------------------------------------------ *)
 subsubsection \<open>All CleanQ RB Invariants\<close>
@@ -287,6 +283,15 @@ lemma frame_weak_x_tl_delta:
   by (metis (no_types, hide_lams) frame frame_rb_weak_x_def rb_delta_tail_incr rb_delta_tail_st_def 
       rb_incr_tail_n_delta_def rb_incr_tail_n_delta_map_def) 
 
+lemma frame_weak_y_tl_delta: 
+  assumes Inv: "CleanQ_RB_Invariants K rb'" and
+          frame: "frame_rb_weak_y rb' rb"
+  shows"map (the \<circ> ring (rTYX rb')) (rb_valid_entries (rTYX rb')) =
+        rb_delta_tail_st (rTYX rb') (rTYX rb) @ map (the \<circ> ring (rTYX rb)) (rb_valid_entries (rTYX rb))"
+  unfolding rb_delta_tail_st_def rb_incr_tail_n_delta_map_def rb_incr_tail_n_delta_def
+  by (metis (no_types, hide_lams) frame frame_rb_weak_y_def rb_delta_tail_incr rb_delta_tail_st_def 
+      rb_incr_tail_n_delta_def rb_incr_tail_n_delta_map_def) 
+
 lemma frame_weak_x_hd_delta:
   assumes Inv: "CleanQ_RB_Invariants K rb'" and
           frame: "frame_rb_weak_x rb' rb"
@@ -296,6 +301,16 @@ lemma frame_weak_x_hd_delta:
   using frame rb_delta_head_incr unfolding frame_rb_weak_x_def
   by (metis rb_delta_head_st_def rb_incr_head_n_delta_def rb_incr_head_n_delta_map_def) 
 
+
+lemma frame_weak_y_hd_delta:
+  assumes Inv: "CleanQ_RB_Invariants K rb'" and
+          frame: "frame_rb_weak_y rb' rb"
+  shows"map (the \<circ> ring (rTXY rb')) (rb_valid_entries (rTXY rb')) @ rb_delta_head_st (rTXY rb') (rTXY rb) =
+        map (the \<circ> ring (rTXY rb)) (rb_valid_entries (rTXY rb))"
+  unfolding rb_delta_head_st_def rb_incr_head_n_delta_map_def rb_incr_head_n_delta_def
+  using frame rb_delta_head_incr unfolding frame_rb_weak_y_def
+  by (metis rb_delta_head_st_def rb_incr_head_n_delta_def rb_incr_head_n_delta_map_def) 
+
 lemma frame_weak_x_sy_delta:
   assumes Inv: "CleanQ_RB_Invariants K rb'" and
           frame: "frame_rb_weak_x rb' rb"
@@ -303,7 +318,31 @@ lemma frame_weak_x_sy_delta:
   using frame unfolding frame_rb_weak_x_def
   by linarith
 
+lemma frame_weak_y_sx_delta:
+  assumes Inv: "CleanQ_RB_Invariants K rb'" and
+          frame: "frame_rb_weak_y rb' rb"
+        shows "rSX rb' \<union> set (rb_delta_tail_st (rTYX rb') (rTYX rb)) = set (rb_delta_head_st (rTXY rb') (rTXY rb)) \<union> rSX rb"
+  using frame unfolding frame_rb_weak_y_def
+  by linarith
+
+lemma frame_weak_x_sy:
+  assumes Inv: "CleanQ_RB_Invariants K rb'" and
+          frame: "frame_rb_weak_x rb' rb"
+  shows "(rSY rb) \<inter> set (rb_delta_head_st (rTYX rb') (rTYX rb)) = {}"
+  using frame unfolding frame_rb_weak_x_def
+  by blast
+
+
+lemma frame_weak_y_sy:
+  assumes Inv: "CleanQ_RB_Invariants K rb'" and
+          frame: "frame_rb_weak_y rb' rb"
+  shows "(rSX rb) \<inter> set (rb_delta_head_st (rTXY rb') (rTXY rb)) = {}"
+  using frame unfolding frame_rb_weak_y_def
+  by blast
+
+
 text \<open>Finally we show that the RB weak frame condition refines the List weak frame condition.\<close>
+
 lemma frame_rb_weak_x_list_weak:
   fixes rb rb' K
   assumes I1: "CleanQ_RB_Invariants K rb'"
@@ -323,37 +362,76 @@ proof -
            rSY rb' \<union> set \<delta>aB = set \<delta>Bc \<union> rSY rb \<and>
            map (the \<circ> ring (rTYX rb')) (rb_valid_entries (rTYX rb')) @ \<delta>Bc = map (the \<circ> ring (rTYX rb)) (rb_valid_entries (rTYX rb)) \<and> rSY rb \<inter> set \<delta>Bc = {} \<and> distinct \<delta>Bc)"
   using frame unfolding frame_rb_weak_x_def frame_rb_weak_left_def
-proof
-
-  define \<delta>xy where "\<delta>xy = rb_delta_tail_st (rTXY rb') (rTXY rb)"
-  define \<delta>yx where "\<delta>yx = rb_delta_head_st (rTYX rb') (rTYX rb)"
-
-  have c1: "map (the \<circ> ring (rTXY rb')) (rb_valid_entries (rTXY rb')) = \<delta>xy @ map (the \<circ> ring (rTXY rb)) (rb_valid_entries (rTXY rb))"
-    using I1 \<delta>xy_def frame frame_weak_x_tl_delta by blast
-
-  have c2: "map (the \<circ> ring (rTYX rb')) (rb_valid_entries (rTYX rb')) @ \<delta>yx = map (the \<circ> ring (rTYX rb)) (rb_valid_entries (rTYX rb))"
-    using I1 \<delta>yx_def frame frame_weak_x_hd_delta by blast
+  proof
+    define \<delta>xy where "\<delta>xy = rb_delta_tail_st (rTXY rb') (rTXY rb)"
+    define \<delta>yx where "\<delta>yx = rb_delta_head_st (rTYX rb') (rTYX rb)"
   
-  have c3: "rSY rb' \<union> set \<delta>xy = set \<delta>yx \<union> rSY rb "
-    using I1 \<delta>xy_def \<delta>yx_def frame frame_weak_x_sy_delta by blast 
-
-  from \<delta>xy_def have s1: "set \<delta>xy \<subseteq> set (CleanQ_RB_list(rTXY rb'))"
-    apply simp unfolding rb_delta_tail_st_def rb_incr_tail_n_delta_map_def
-    by (simp add: CleanQ_RB_list_def c1)
+    have c1: "map (the \<circ> ring (rTXY rb')) (rb_valid_entries (rTXY rb')) = \<delta>xy @ map (the \<circ> ring (rTXY rb)) (rb_valid_entries (rTXY rb))"
+      using I1 \<delta>xy_def frame frame_weak_x_tl_delta by blast
   
-  from \<delta>yx_def have s2: "set \<delta>yx \<subseteq> set (CleanQ_RB_list(rTYX rb))"
-    apply simp unfolding rb_delta_head_st_def rb_incr_head_n_delta_map_def
-    by (metis CleanQ_RB_list_def Un_upper2 c2 set_append)
-     
-  have c4: "rSY rb \<inter> set \<delta>yx = {}"
-    sorry
-  
-  from I1 have c5: "distinct \<delta>yx"
-    using \<delta>yx_def frame frame_rb_weak_x_def by blast 
+    have c2: "map (the \<circ> ring (rTYX rb')) (rb_valid_entries (rTYX rb')) @ \<delta>yx = map (the \<circ> ring (rTYX rb)) (rb_valid_entries (rTYX rb))"
+      using I1 \<delta>yx_def frame frame_weak_x_hd_delta by blast
     
-  show ?thesis using c1 c2 c3 c4 c5
-    by blast
+    have c3: "rSY rb' \<union> set \<delta>xy = set \<delta>yx \<union> rSY rb "
+      using I1 \<delta>xy_def \<delta>yx_def frame frame_weak_x_sy_delta by blast 
+  
+    from I1 have c4: "distinct \<delta>yx"
+      using \<delta>yx_def frame frame_rb_weak_x_def by blast 
+  
+    from \<delta>yx_def frame have c5: "rSY rb \<inter> set \<delta>yx = {}" 
+      unfolding frame_rb_weak_x_def
+      by blast 
+    
+    show ?thesis using c1 c2 c3 c4 c5
+      by blast
+  qed
 qed
+
+lemma frame_rb_weak_y_list_weak:
+  fixes rb rb' K
+  assumes I1: "CleanQ_RB_Invariants K rb'"
+      and frame: "frame_rb_weak_y rb' rb"
+    shows "frame_list_weak (lTYX (CleanQ_RB2List rb'), lSX (CleanQ_RB2List rb'), lTXY (CleanQ_RB2List rb'), lSY (CleanQ_RB2List rb')) 
+                           (lTYX (CleanQ_RB2List rb), lSX (CleanQ_RB2List rb), lTXY (CleanQ_RB2List rb), lSY (CleanQ_RB2List rb))"
+  unfolding CleanQ_RB2List_def CleanQ_RB_list_def
+  apply auto 
+proof -
+  show "\<And>x. x \<in> rSY rb' \<Longrightarrow> x \<in> rSY rb"
+    by (metis frame frame_rb_weak_y_def) 
+  show " \<And>x. x \<in> rSY rb \<Longrightarrow> x \<in> rSY rb'"
+    by (metis frame frame_rb_weak_y_def)
+  show "\<exists>\<delta>aB::'a list.
+       map (the \<circ> ring (rTYX rb')) (rb_valid_entries (rTYX rb')) = \<delta>aB @ map (the \<circ> ring (rTYX rb)) (rb_valid_entries (rTYX rb)) \<and>
+       (\<exists>\<delta>Bc::'a list.
+           rSX rb' \<union> set \<delta>aB = set \<delta>Bc \<union> rSX rb \<and>
+           map (the \<circ> ring (rTXY rb')) (rb_valid_entries (rTXY rb')) @ \<delta>Bc = map (the \<circ> ring (rTXY rb)) (rb_valid_entries (rTXY rb)) \<and> rSX rb \<inter> set \<delta>Bc = {} \<and> distinct \<delta>Bc)"
+  using frame unfolding frame_rb_weak_y_def frame_rb_weak_left_def
+  proof
+  
+    define \<delta>xy where "\<delta>xy = rb_delta_tail_st (rTYX rb') (rTYX rb)"
+    define \<delta>yx where "\<delta>yx = rb_delta_head_st (rTXY rb') (rTXY rb)"
+  
+    have c1: "map (the \<circ> ring (rTYX rb')) (rb_valid_entries (rTYX rb')) = \<delta>xy @ map (the \<circ> ring (rTYX rb)) (rb_valid_entries (rTYX rb))"
+      using I1 \<delta>xy_def frame frame_weak_y_tl_delta by blast
+  
+    have c2: "map (the \<circ> ring (rTXY rb')) (rb_valid_entries (rTXY rb')) @ \<delta>yx = map (the \<circ> ring (rTXY rb)) (rb_valid_entries (rTXY rb))"
+      using I1 \<delta>yx_def frame frame_weak_y_hd_delta by blast
+    
+    have c3: "rSX rb' \<union> set \<delta>xy = set \<delta>yx \<union> rSX rb "
+      using I1 \<delta>xy_def \<delta>yx_def frame frame_weak_y_sx_delta by blast 
+  
+    from I1 have c4: "distinct \<delta>yx"
+      using \<delta>yx_def frame frame_rb_weak_y_def by blast 
+  
+    from \<delta>yx_def frame have c5: "rSX rb \<inter> set \<delta>yx = {}" 
+      unfolding frame_rb_weak_y_def
+      by blast 
+    
+    show ?thesis using c1 c2 c3 c4 c5
+      by blast
+  qed
+qed
+
 
 (* ==================================================================================== *)
 subsection \<open>State Transition Operations\<close>
